theories/iris_examples.v
@@ -1,8 +1,9 @@
 From mathcomp Require Import ssreflect eqtype seq ssrbool.
 From iris.program_logic Require Import language.
-From iris.proofmode Require Import tactics.
-From iris.program_logic Require Export weakestpre lifting.
-From iris.base_logic Require Export gen_heap proph_map.
+From iris.proofmode Require Import base tactics classes.
+From iris.base_logic Require Export gen_heap ghost_map proph_map.
+From iris.base_logic.lib Require Export fancy_updates.
+From iris.bi Require Export weakestpre.
 Require Export iris iris_locations iris_properties iris_atomicity stdpp_aux.
 Require Export iris_use.
 Require Export datatypes host operations properties opsem.
@@ -13,33 +14,98 @@ Unset Printing Implicit Defensive.
 
 Close Scope byte_scope.
 
-Let expr := iris.expr.
-Let val := iris.val.
-Let to_val := iris.to_val.
+Let expr := iris_use.expr.
+Let val := iris_use.val.
+Let to_val := iris_use.to_val.
 
 (* Example Programs *)
 Section Examples.
-
-Context `{!wfuncG host_function Σ, !wtabG Σ, !wmemG Σ, !wmemsizeG Σ, !wglobG Σ, !wlocsG Σ, !winstG Σ(*, irisG (wasm_lang host_function host_instance) Σ*)}.
+  
+Import DummyHosts.
+  (*
+Variable host_function : eqType.
 
 Let host := host.host host_function.
 Let function_closure := function_closure host_function.
 Let store_record := store_record host_function.
 
-Variable host_instance: host.
-
+Variable host_instance : host.
+*)
 Let reduce := @reduce host_function host_instance.
-
 
 (*
 Let wasm_mixin : LanguageMixin _ _ _ := wasm_mixin host_instance.
-
+ *)
 Canonical Structure wasm_lang := Language wasm_mixin.
 
 Let reducible := @reducible wasm_lang.
 
-Let prim_step := @iris.prim_step host_function host_instance.
-*)
+Context `{!wfuncG Σ, !wtabG Σ, !wmemG Σ, !wmemsizeG Σ, !wglobG Σ, !wframeG Σ}.
+
+(* TODO: Resolve duplicated notations *)
+Notation "n ↦[wf]{ q } v" := (mapsto (L:=N) (V:=function_closure) n q v%V)
+                           (at level 20, q at level 5, format "n ↦[wf]{ q } v") : bi_scope.
+Notation "n ↦[wf] v" := (mapsto (L:=N) (V:=function_closure) n (DfracOwn 1) v%V)
+                      (at level 20, format "n ↦[wf] v") : bi_scope.
+Notation "n ↦[wt]{ q } [ i ] v" := (mapsto (L:=N*N) (V:=funcelem) (n, i) q v%V)
+                           (at level 20, q at level 5, format "n ↦[wt]{ q } [ i ] v") : bi_scope.
+Notation "n ↦[wt][ i ] v" := (mapsto (L:=N*N) (V:=funcelem) (n, i) (DfracOwn 1) v%V)
+                      (at level 20, format "n ↦[wt][ i ] v") : bi_scope.
+Notation "n ↦[wm]{ q } [ i ] v" := (mapsto (L:=N*N) (V:=byte) (n, i) q v%V)
+                           (at level 20, q at level 5, format "n ↦[wm]{ q } [ i ] v") : bi_scope.
+Notation "n ↦[wm][ i ] v" := (mapsto (L:=N*N) (V:=byte) (n, i) (DfracOwn 1) v% V)
+                           (at level 20, format "n ↦[wm][ i ] v") : bi_scope.
+Notation "n ↦[wmlength] v" := (mapsto (L:=N) (V:=N) n (DfracOwn 1) v% V)
+                           (at level 20, format "n ↦[wmlength] v") : bi_scope.
+Notation "n ↦[wg]{ q } v" := (mapsto (L:=N) (V:=global) n q v%V)
+                           (at level 20, q at level 5, format "n ↦[wg]{ q } v").
+Notation "n ↦[wg] v" := (mapsto (L:=N) (V:=global) n (DfracOwn 1) v%V)
+                      (at level 20, format "n ↦[wg] v") .
+Notation " ↪[frame]{ q } v" := (ghost_map_elem frameGName tt q v%V)
+                           (at level 20, q at level 5, format " ↪[frame]{ q } v") .
+Notation " ↪[frame] v" := (ghost_map_elem frameGName tt (DfracOwn 1) v%V)
+                           (at level 20, format " ↪[frame] v").
+
+Notation "'WP' e @ s ; E 'CTX' i ; lh {{ Φ } }" := (wp_wasm_ctx s E e%E Φ i lh)
+  (at level 20, e, Φ, lh at level 200, only parsing) : bi_scope.
+Notation "'WP' e @ E 'CTX' i ; lh {{ Φ } }" := (wp_wasm_ctx NotStuck E e%E Φ i lh)
+  (at level 20, e, Φ, lh at level 200, only parsing) : bi_scope.
+Notation "'WP' e @ E 'CTX' i ; lh ? {{ Φ } }" := (wp_wasm_ctx MaybeStuck E e%E Φ i lh)
+  (at level 20, e, Φ, lh at level 200, only parsing) : bi_scope.
+Notation "'WP' e 'CTX' i ; lh {{ Φ } }" := (wp_wasm_ctx NotStuck ⊤ e%E Φ i lh)
+  (at level 20, e, Φ, lh at level 200, only parsing) : bi_scope.
+Notation "'WP' e 'CTX' i ; lh ? {{ Φ } }" := (wp_wasm_ctx MaybeStuck ⊤ e%E Φ i lh)
+  (at level 20, e, Φ, lh at level 200, only parsing) : bi_scope.
+Notation "'WP' e @ s ; E 'CTX_EMPTY' {{ Φ } }" := (wp_wasm_ctx s E e%E Φ 0 (LH_base [] []))
+  (at level 20, e, Φ at level 200, only parsing) : bi_scope.
+
+
+Notation "'WP' e @ s ; E 'CTX' i ; lh {{ v , Q } }" := (wp_wasm_ctx s E e%E (λ v, Q) i lh)
+  (at level 20, e, Q, lh at level 200,
+   format "'[hv' 'WP'  e  '/' @  '[' s ;  '/' E  ']' 'CTX'  '/' '[' i ;  '/' lh ']'  '/' {{  '[' v ,  '/' Q  ']' } } ']'") : bi_scope.
+Notation "'WP' e @ s ; E 'CTX_EMPTY' {{ v , Q } }" := (wp_wasm_ctx s E e%E (λ v, Q) 0 (LH_base [] []))
+  (at level 20, e, Q at level 200,
+   format "'[hv' 'WP'  e  '/' @  '[' s ;  '/' E  ']' 'CTX_EMPTY'  '/' {{  '[' v ,  '/' Q  ']' } } ']'") : bi_scope.
+Notation "'WP' e @ E 'CTX' i ; lh {{ v , Q } }" := (wp_wasm_ctx NotStuck E e%E (λ v, Q) i lh)
+  (at level 20, e, Q, lh at level 200,
+   format "'[hv' 'WP'  e  '/' @ '[' E  '/' ']' 'CTX'  '/' '[' i ;  '/' lh ']'  '/' {{  '[' v ,  '/' Q  ']' } } ']'") : bi_scope.
+Notation "'WP' e @ E 'CTX' i ; lh ? {{ v , Q } }" := (wp_wasm_ctx MaybeStuck E e%E (λ v, Q) i lh)
+  (at level 20, e, Q, lh at level 200,
+   format "'[hv' 'WP'  e  '/' @  '[' E  '/' ']' 'CTX'  '/' '[' i ;  '/' lh ']'  '/' ? {{  '[' v ,  '/' Q  ']' } } ']'") : bi_scope.
+Notation "'WP' e 'CTX' i ; lh {{ v , Q } }" := (wp_wasm_ctx NotStuck ⊤ e%E (λ v, Q) i lh)
+  (at level 20, e, Q, lh at level 200,
+   format "'[hv' 'WP'  e  '/' 'CTX'  '/' '[' i ;  '/' lh ']'  '/' {{  '[' v ,  '/' Q  ']' } } ']'") : bi_scope.
+Notation "'WP' e 'CTX' i ; lh ? {{ v , Q } }" := (wp_wasm_ctx MaybeStuck ⊤ e%E (λ v, Q) i lh)
+  (at level 20, e, Q, lh at level 200,
+   format "'[hv' 'WP'  e '/' 'CTX'  '/' '[' i ;  '/' lh ']'  '/' ? {{  '[' v ,  '/' Q  ']' } } ']'") : bi_scope.
+
+
+Notation "'WP' e @ s ; E 'FRAME' n ; f {{ Φ } }" := (wp_wasm_frame s E e%E Φ n f)
+  (at level 20, only parsing) : bi_scope.
+
+Notation "'WP' e @ s ; E 'FRAME' n ; f {{ v , Q } }" := (wp_wasm_frame s E e%E (λ v, Q) n f)
+  (at level 20, e, Q, n, f at level 200,
+   format "'[hv' 'WP'  e  '/' @  '[' s ;  '/' E  ']' 'FRAME'  '/' '[' n ; f ']'  '/' {{  '[' v ,  '/' Q  ']' } } ']'") : bi_scope.
 
 Definition xx i := (VAL_int32 (Wasm_int.int_of_Z i32m i)).
 Definition xb b := (VAL_int32 (wasm_bool b)).
@@ -49,11 +115,10 @@ Definition my_add : expr :=
      AI_basic (BI_const (xx 2));
   AI_basic (BI_binop T_i32 (Binop_i BOI_add))].
 
-(* Doesn't work yet -- there are some typeclass and context bugs to be fixed *)
-Lemma myadd_spec (s : stuckness) (E : coPset) (Φ: val -> iProp Σ) : 
-  Φ (immV [xx 5]) ⊢ WP my_add @ s; E {{ v, Φ v }}.
+Lemma myadd_spec (s : stuckness) (E : coPset) (Φ: val -> iProp Σ) (f0: frame): 
+  ↪[frame] f0 -∗ Φ (immV [xx 5]) -∗ WP my_add @ s; E {{ v, Φ v ∗  ↪[frame] f0  }}.
 Proof.
-  iIntros "HΦ".
+  iIntros "HP".
   unfold my_add.
   by iApply wp_binop.
 Qed.
@@ -66,17 +131,17 @@ Definition my_add2: expr :=
   AI_basic (BI_const (xx 2));
   AI_basic (BI_binop T_i32 (Binop_i BOI_add))].
 
-Lemma myadd2_spec (s : stuckness) (E : coPset) (Φ: val -> iProp Σ) :
-  Φ (immV [xx 5]) ⊢ WP my_add2 @ s; E {{ v, Φ v }}.
+Lemma myadd2_spec (s : stuckness) (E : coPset) (Φ: val -> iProp Σ) f0:
+  ↪[frame] f0 -∗ Φ (immV [xx 5]) -∗ WP my_add2 @ s; E {{ v, Φ v ∗ ↪[frame] f0 }}.
 Proof.
-  iIntros "HΦ".
+  iIntros "Hf0 HΦ".
   replace my_add2 with (take 3 my_add2 ++ drop 3 my_add2) => //.
   iApply wp_seq => /=.
-  instantiate (1 := fun v => (⌜ v = immV [xx 3] ⌝)%I ).
-  iSplit => //.
-  iSplitR "HΦ"; first by iApply wp_binop.
-  iIntros (? ->) => /=.
-  by iApply wp_binop.
+  instantiate (1 := fun v => (⌜ v = immV [xx 3] ⌝ ∗ ↪[frame] f0)%I ).
+  iSplitL ""; first by iIntros "(%H & ?)".
+  iSplitL "Hf0"; first by iApply (wp_binop with "[$]") => //.
+  iIntros (?) "(-> & Hf0)" => /=.
+  by iApply (wp_binop with "[$]").
 Qed.
 
 (* --------------------------------------------------------------------------------------------- *)
@@ -115,17 +180,19 @@ Ltac take_drop_app_rewrite_twice n m :=
   end.
 
 (* Examples of blocks that return normally *)
-Lemma label_check_easy :
+Lemma label_check_easy f0:
+  ↪[frame] f0
   ⊢ WP [::AI_basic
          (BI_block (Tf [] [T_i32;T_i32])
-            [::BI_const (xx 2); BI_const (xx 3)] )] {{ λ v, ⌜v = immV [xx 2;xx 3]⌝ }}.
+            [::BI_const (xx 2); BI_const (xx 3)] )] {{ λ v, ⌜v = immV [xx 2;xx 3]⌝ ∗ ↪[frame] f0}}.
 Proof.
   rewrite -iRewrite_nil_l.
-  iApply wp_block;eauto. iNext.
+  iIntros "Hf0"; iApply (wp_block with "[$]");eauto. iNext.
+  iIntros "Hf0".
   iApply wp_wasm_empty_ctx.
   iApply wp_label_push_nil. simpl.
-  iApply wp_val_return;auto.
-  iApply wp_value;eauto. done.
+  iApply (wp_val_return with "[$]");auto.
+  iIntros "Hf0"; iApply wp_value;eauto. done.
 Qed.
 Lemma label_check_easy' :
   ⊢ WP [::AI_basic
